# baseURI: http://publications.europa.eu/ontology/euvoc
# imports: http://publications.europa.eu/ontology/euvoc/externalImports
# imports: http://publications.europa.eu/ontology/euvoc/internalImports
# prefix: euvoc

@prefix : <http://publications.europa.eu/ontology/euvoc#> .
@prefix adms: <http://www.w3.org/ns/adms#> .
@prefix cc: <http://creativecommons.org/ns#> .
@prefix cdm: <http://publications.europa.eu/ontology/cdm#> .
@prefix cmr: <http://publications.europa.eu/ontology/cdm/cmr#> .
@prefix dataTypeDefinitions: <http://publications.europa.eu/ontology/euvoc/dataTypeDefinitions#> .
@prefix dc: <http://purl.org/dc/elements/1.1/> .
@prefix dcam: <http://purl.org/dc/dcam/> .
@prefix dcat: <http://www.w3.org/ns/dcat#> .
@prefix dcmitype: <http://purl.org/dc/dcmitype/> .
@prefix dct: <http://purl.org/dc/terms/> .
@prefix dcterms: <http://purl.org/dc/terms/> .
@prefix dctype: <http://purl.org/dc/dcmitype/> .
@prefix eli: <http://data.europa.eu/eli/ontology#> .
@prefix euvoc: <http://publications.europa.eu/ontology/euvoc#> .
@prefix event: <http://purl.org/NET/c4dm/event.owl#> .
@prefix extensionDesctiptions: <http://publications.europa.eu/ontology/euvoc/extensionDesctiptions#> .
@prefix externalImports: <http://publications.europa.eu/ontology/euvoc/externalImports#> .
@prefix foaf: <http://xmlns.com/foaf/0.1/> .
@prefix geosparql: <http://www.opengis.net/ont/geosparql#> .
@prefix geosparqlsf: <http://www.opengis.net/ont/sf#> .
@prefix geowgs84: <http://www.w3.org/2003/01/geo/wgs84_pos#> .
@prefix gml: <http://www.opengis.net/ont/gml#> .
@prefix legalDescriptions: <http://publications.europa.eu/ontology/euvoc/legalDescriptions> .
@prefix lemon: <http://lemon-model.net/lemon#> .
@prefix lexinfo: <http://www.lexinfo.net/ontology/2.0/lexinfo#> .
@prefix linguisticDescriptions: <http://publications.europa.eu/ontology/euvoc/linguisticDescriptions#> .
@prefix locn: <http://www.w3.org/ns/locn#> .
@prefix lvont: <http://lexvo.org/ontology#> .
@prefix org: <http://www.w3.org/ns/org#> .
@prefix owl: <http://www.w3.org/2002/07/owl#> .
@prefix person: <http://www.w3.org/ns/person#> .
@prefix pim: <http://www.w3.org/2000/10/swap/pim/contact#> .
@prefix prov: <http://www.w3.org/ns/prov#> .
@prefix rdaelements: <http://rdaregistry.info/Elements/c/> .
@prefix rdakit: <http://metadataregistry.org/uri/profile/rdakit/> .
@prefix rdf: <http://www.w3.org/1999/02/22-rdf-syntax-ns#> .
@prefix rdfs: <http://www.w3.org/2000/01/rdf-schema#> .
@prefix schema: <http://schema.org/> .
@prefix skos: <http://www.w3.org/2004/02/skos/core#> .
@prefix skosxl: <http://www.w3.org/2008/05/skos-xl#> .
@prefix spatialDescriptions: <http://publications.europa.eu/ontology/euvoc/spatialDescriptions#> .
@prefix spin: <http://spinrdf.org/spin#> .
@prefix tableDescriptions: <http://publications.europa.eu/ontology/euvoc/tableDescriptions#> .
@prefix temporalDescriptions: <http://publications.europa.eu/ontology/euvoc/temporalDescriptions#> .
@prefix terms: <http://purl.org/dc/terms/> .
@prefix time: <http://www.w3.org/2006/time#> .
@prefix vann: <http://purl.org/vocab/vann/> .
@prefix vcard: <http://www.w3.org/2006/vcard/ns#> .
@prefix voaf: <http://purl.org/vocommons/voaf#> .
@prefix void: <http://rdfs.org/ns/void#> .
@prefix xsd: <http://www.w3.org/2001/XMLSchema#> .

<http://publications.europa.eu/ontology/euvoc>
  rdf:type owl:Ontology ;
  rdfs:comment """Euvoc ontology defines a set of properties used to enrich skos, org and dcat ontologies. 

Properties defined in Euvoc are used by:
- skos Publications Office application profile (SKOS-AP-EU) 
- org Publications Office application profile (ORG-AP-OP) 
- dcat Publications Office application profile (DCAT-AP-OP)
- cdm ontology used for the CELLAR. The euvoc ontology is imported in cdm ontology starting on version 4 of the cdm ontology"""@en ;
  rdfs:comment """v1.00 alpha 1 to V1.00 alpha 2
1) org:classification has a range: OrganizationType
2) euvoc:xlType change to euvoc:xlClassification

v1.00 alpha 2 to V1.00 alpha 3
1) property prov:hadPrimarySource not use any more, use dct:source instead
2) property euvoc:thesStatus is renamed euvoc:status (used for skos:Concept and skos-xl:Label)
3) property iso:status is added,  euvoc:status (used for skos:Concept and skos-xl:Label)
4) use euvoc:endDate instead prov:invalidatedAtTime 
5) use euvoc:startDate instead of prov:generatedAtTime 
6) foaf:img is removed from org:Organization, use foaf:depiction instead

v1.00 alpha 3 to V1.00 2015/05/06
1) iso:status is suppressed, we use euvoc:status
2) http://publications.europa.eu/resource/authority/grammatical-gender is declared as the sexuel gender table and made equivalent to class gender instead of sdmx:sex
3) dct:creator is suppressed as object property, it was already declared as data property

V1.00 to V1.01 2015/05/08
1) correct a mistake on a euvoc restriction which was express in the org ontology intead of euvoc
2) suppress the issued date of the euvoc ontology in the metadata of the ontology

V1.01 to V1.02 2015/05/08
http://publications.europa.eu/resource/authority/license changed to  http://publications.europa.eu/resource/authority/licence (name of a MDR authority)

V1.02 to V1.03 2015/7/14
correct mistakes : Concept was declared as equivalent to \"Frequency\" and Concept had cdm subclasses : both were removed

V1.03 to V1.04 2015/7/15
adding data property endDate and startDate to skos-xl:Label
delete decrecated classes from vcard ontology. Change the uri of the classes which were defined in cdm namespace to give them a uri in euvoc namespace (corporate, country, place, concept-eurovoc, language). Change on Site class which was defined as a subclass of Document when it is a subclass of Thing.

V1.04 to V1.05 2015/7/15
added euvoc:startDate and euvoc:endDate to org:Membership instead of Prov properties

V1.05 to V1.06 2015/07/17
because of extreme delays (up to ~2 hours) during the inference with Pellet
we removed on skos:Concept and vcard:Kind, but also anywere else the constraint on properties which used owl:onDataRange. To do this the data type is assigned to rdfs:Literal for all the property constraints.

V1.06 to V1.07 2015/07/24
-euvoc:license property replaces dcterms:license property
-euvoc:contributor property replaces dcterms:contributor
-suppression of dcterms properties declaration when they were both declared as annotation and data of object property
-euvoc does not import void, dcterms, adms ontologies any more, classes and property are redeclared inside euvoc, to avoid potential conflicts coming from those ontologies

v1.07 to V1.08 2015/07/29
-class Domain changed to DomainEuroVoc
-ConceptScheme are classified with the property euvoc:domain range DomainEuroVoc
-Range of dcat:theme is now EuroVoc waiting for the final MDR table

v1.08 to V1.09 2015/10/09
- Creation of the class DatasetTheme, subclass of skos:Concept, equivalent to MDR table dataset-theme
- Range of dcat:theme is now DatasetTheme {@en}

v1.09    euvoc.rdf 2015-10-09
- the state before the redesign

v1.1 2016-09-01
- split of the ontology into modules: spatialDescription, temporalDescription, linguisticDescription, tableDescription, tableImports and extensionDescription 
- fuirther extended with SHACL Shapes in another ontology """ ;
  rdfs:label "EuVoc Ontology" ;
  owl:imports <http://publications.europa.eu/ontology/euvoc/externalImports> ;
  owl:imports <http://publications.europa.eu/ontology/euvoc/internalImports> ;
  owl:versionIRI <http://publications.europa.eu/ontology/euvoc#1.1> ;
  owl:versionInfo "EuVoc 1.1" ;
.
euvoc:XlNotation
  rdf:type owl:Class ;
  rdfs:comment "Current value and historical values of skos:notation."@en ;
  rdfs:label "Notation (reified SKOS notation)" ;
  rdfs:subClassOf [
      rdf:type owl:Restriction ;
      owl:maxCardinality "1"^^xsd:nonNegativeInteger ;
      owl:onProperty euvoc:endDate ;
    ] ;
  rdfs:subClassOf [
      rdf:type owl:Restriction ;
      owl:maxCardinality "1"^^xsd:nonNegativeInteger ;
      owl:onProperty euvoc:startDate ;
    ] ;
  rdfs:subClassOf [
      rdf:type owl:Restriction ;
      owl:maxQualifiedCardinality "1"^^xsd:nonNegativeInteger ;
      owl:onClass euvoc:ConceptStatus ;
      owl:onProperty euvoc:status ;
    ] ;
  owl:equivalentClass [
      rdf:type owl:Class ;
      owl:intersectionOf (
          [
            rdf:type owl:Restriction ;
            owl:maxCardinality "1"^^xsd:nonNegativeInteger ;
            owl:onProperty euvoc:xlCodification ;
          ]
          [
            rdf:type owl:Restriction ;
            owl:minCardinality "1"^^xsd:nonNegativeInteger ;
            owl:onProperty euvoc:xlCodification ;
          ]
        ) ;
    ] ;
.
euvoc:XlNote
  rdf:type owl:Class ;
  rdfs:comment "Current value and historical values of skos:note"@en ;
  rdfs:label "Note (reified SKOS note)" ;
  rdfs:subClassOf [
      rdf:type owl:Restriction ;
      owl:maxCardinality "1"^^xsd:nonNegativeInteger ;
      owl:onProperty euvoc:endDate ;
    ] ;
  rdfs:subClassOf [
      rdf:type owl:Restriction ;
      owl:maxCardinality "1"^^xsd:nonNegativeInteger ;
      owl:onProperty euvoc:startDate ;
    ] ;
.
euvoc:XlNumericalValue
  rdf:type owl:Class ;
  rdfs:comment "Current value and historical values of numerical properties. Used to store current and historical values of euvoc:protocolLevel"@en ;
  rdfs:label "Numeric Value (Deprecated)" ;
  rdfs:subClassOf [
      rdf:type owl:Restriction ;
      owl:maxCardinality "1"^^xsd:nonNegativeInteger ;
      owl:onProperty euvoc:endDate ;
    ] ;
  rdfs:subClassOf [
      rdf:type owl:Restriction ;
      owl:maxCardinality "1"^^xsd:nonNegativeInteger ;
      owl:onProperty euvoc:startDate ;
    ] ;
  owl:deprecated "true"^^xsd:boolean ;
.
euvoc:XlSemanticRelation
  rdf:type owl:Class ;
  rdfs:comment "Current value and historical values of org:hasSubOrganization"@en ;
  rdfs:label "Semantic Relation (Deprecated)" ;
  rdfs:subClassOf [
      rdf:type owl:Restriction ;
      owl:maxCardinality "1"^^xsd:nonNegativeInteger ;
      owl:onProperty euvoc:endDate ;
    ] ;
  rdfs:subClassOf [
      rdf:type owl:Restriction ;
      owl:maxCardinality "1"^^xsd:nonNegativeInteger ;
      owl:onProperty euvoc:startDate ;
    ] ;
  owl:deprecated "true"^^xsd:boolean ;
.
euvoc:XlType
  rdf:type owl:Class ;
  rdfs:comment "Current value and historical values of org:classification."@en ;
  rdfs:subClassOf [
      rdf:type owl:Restriction ;
      owl:maxCardinality "1"^^xsd:nonNegativeInteger ;
      owl:onProperty euvoc:endDate ;
    ] ;
  rdfs:subClassOf [
      rdf:type owl:Restriction ;
      owl:maxCardinality "1"^^xsd:nonNegativeInteger ;
      owl:onProperty euvoc:startDate ;
    ] ;
.
euvoc:adoptedEuroCurrencyOn
  rdf:type owl:DatatypeProperty ;
  rdfs:comment "adopted euro currency on" ;
  rdfs:label "adopted euro currency on" ;
  rdfs:range xsd:date ;
  owl:versionInfo "EuVoc 1.1" ;
.
euvoc:contactPoint
  rdf:type owl:ObjectProperty ;
  rdfs:comment "This relationship is mainly designed for WhoIsWho but is also used in MDR NALs." ;
  rdfs:comment "a relationship ascribing a contact point, usually of the vacrd:Kind type, to an org entity of site, membership or organization types." ;
  rdfs:label "contact point" ;
  owl:versionInfo "EuVoc 1.1" ;
.
euvoc:context
  rdf:type owl:ObjectProperty ;
  rdfs:comment "context" ;
  rdfs:label "context" ;
  skos:prefLabel "context" ;
.
euvoc:contributor
  rdf:type owl:ObjectProperty ;
.
euvoc:domain
  rdf:type owl:ObjectProperty ;
  rdfs:comment "To indicate the subject of the controlled vocabulary based on the Domain vocabulary, part of EuroVoc"@en ;
  rdfs:domain skos:ConceptScheme ;
  rdfs:range euvoc:DomainEurovoc ;
.
euvoc:downloadURL
  rdf:type owl:ObjectProperty ;
  rdfs:range rdfs:Resource ;
.
euvoc:endDate
  rdf:type owl:DatatypeProperty ;
  rdfs:comment "Date ending a period of time."@en ;
.
euvoc:getsReportingFrom
  rdf:type owl:ObjectProperty ;
  rdfs:comment "indicates from who the person gets reporting from."@en ;
  rdfs:range org:Membership ;
  owl:inverseOf euvoc:reportsTo ;
.
euvoc:inhabitantNameForm
  rdf:type owl:ObjectProperty ;
  rdfs:comment "indicates the relation between  an inhabitant name form and the noun of the place they live in. Both are instances of skosxl:Label."@en ;
.
euvoc:isTextual
  rdf:type owl:DatatypeProperty ;
  rdfs:comment "is textual" ;
  rdfs:domain terms:FileFormat ;
  rdfs:label "is textual" ;
  rdfs:range xsd:boolean ;
  owl:versionInfo "EuVoc 1.1" ;
.
euvoc:licenceVersion
  rdf:type owl:DatatypeProperty ;
  rdfs:comment "licence version is intended to express the version of the licences from Licences NAL" ;
  rdfs:label "licence version" ;
  rdfs:range xsd:string ;
  owl:versionInfo "EuVoc 1.1" ;
.
euvoc:license
  rdf:type owl:ObjectProperty ;
  rdfs:range terms:LicenseDocument ;
.
euvoc:managedBy
  rdf:type owl:ObjectProperty ;
  rdfs:comment "relates a site to the organization which manages it" ;
  rdfs:domain org:Site ;
  rdfs:label "managed by" ;
  rdfs:range org:Organization ;
  owl:versionInfo "EuVoc 1.1" ;
.
euvoc:officeAddress
  rdf:type owl:DatatypeProperty ;
  rdfs:comment "address of the office inside the building. Subproperty of vcard:street-address"@en ;
  rdfs:subPropertyOf vcard:street-address ;
.
euvoc:officialBirthName
  rdf:type owl:DatatypeProperty ;
  rdfs:comment "Mainly to manage name of the person before marriage. In the original script."@en ;
.
euvoc:officialFamilyName
  rdf:type owl:DatatypeProperty ;
  rdfs:comment "The family name of some person.  In the original script."@en ;
.
euvoc:officialGivenName
  rdf:type owl:DatatypeProperty ;
  rdfs:comment "The given name of some person. In the original script."@en ;
  rdfs:range rdfs:Literal ;
.
euvoc:officialJournalDate
  rdf:type owl:DatatypeProperty ;
  rdfs:comment "official journal date; originally used in treaties table" ;
  rdfs:label "official journal date" ;
  rdfs:range xsd:date ;
  owl:versionInfo "EuVoc 1.1" ;
.
euvoc:officialJournalNumber
  rdf:type owl:DatatypeProperty ;
  rdfs:comment "official journal number; originally used in treaty table" ;
  rdfs:label "official journal number" ;
  rdfs:range xsd:string ;
  owl:versionInfo "EuVoc 1.1" ;
.
euvoc:officialJournalSeries
  rdf:type owl:DatatypeProperty ;
  rdfs:comment "official journal series; originally used in treaties table" ;
  rdfs:label "official journal series" ;
  rdfs:range xsd:string ;
  owl:versionInfo "EuVoc 1.1" ;
.
euvoc:order
  rdf:type owl:DatatypeProperty ;
  rdfs:comment "Current value of the order of the resource among its siblings"@en ;
  rdfs:range xsd:integer ;
.
euvoc:orderMethod
  rdf:type owl:DatatypeProperty ;
  rdfs:comment "Method used to order the related memberships  and sub-organisations. In 99% of the case the method  is based on the order number, not on alphabetic.xs:simpleType name=\"orderMethod\">, <xs:restriction base=\"xs:string\">, <xs:enumeration value=\"default\"/>, <xs:enumeration value=\"list\"/>, <xs:enumeration value=\"protocolar\"/>, <xs:enumeration value=\"alphabetic\"/>, <xs:enumeration value=\"id\"/>"@en ;
  rdfs:range rdfs:Literal ;
.
euvoc:positionComplement
  rdf:type owl:DatatypeProperty ;
  rdfs:comment "Allows to enrich the position with a free text such as \"to the director\", \"in charge of IT”.."@en ;
  rdfs:range rdfs:Literal ;
.
euvoc:positionStatus
  rdf:type owl:ObjectProperty ;
  rdfs:comment "Allows to enrich the function with a controlled value."@en ;
  rdfs:range euvoc:PositionStatus ;
.
euvoc:protocolLevel
  rdf:type owl:DatatypeProperty ;
  rdfs:comment "Current value of the protocol-level."@en ;
  rdfs:range xsd:integer ;
.
euvoc:reportsTo
  rdf:type owl:ObjectProperty ;
  rdfs:comment "Indicates the reporting link for example between a director and his assistant.Current value."@en ;
  rdfs:range org:Membership ;
.
euvoc:represents
  rdf:type owl:ObjectProperty ;
  rdfs:comment "A person in a membership can represent an agent. i.e. a civil servant represents the state in a board of administration, a deputy represents his country at the parliament."@en ;
  rdfs:range foaf:Agent ;
.
euvoc:roleQualification
  rdf:type owl:ObjectProperty ;
  rdfs:comment "Indicates the type of position of the person. i.e. judge, deputy, director… Some business rules are related to this position, like the retention time of the personal information, the publication or not of some of the properties (you don't publish judge telephone number), the publication of the full given name or just the first letter…."@en ;
  rdfs:range euvoc:RoleQualification ;
.
euvoc:startDate
  rdf:type owl:DatatypeProperty ;
  rdfs:comment "Date starting a period of time."@en ;
.
euvoc:status
  rdf:type owl:ObjectProperty ;
  rdfs:comment "Indicates the status of a skos:Concept or a skosxl:Label, or any resource related to controlled vocabulary management."@en ;
  rdfs:range euvoc:ConceptStatus ;
.
euvoc:xlChangeNote
  rdf:type owl:ObjectProperty ;
  rdfs:comment "This property is a reified version of the skos:changeNote" ;
  rdfs:label "xl change note" ;
  rdfs:range euvoc:XlNote ;
  rdfs:subPropertyOf euvoc:xlNote ;
  skos:prefLabel "xl change note" ;
.
euvoc:xlClassification
  rdf:type owl:ObjectProperty ;
  rdfs:comment "Relates a resource to the historical values of org:classification."@en ;
  rdfs:domain org:Organization ;
  rdfs:range euvoc:XlType ;
.
euvoc:xlCodification
  rdf:type owl:DatatypeProperty ;
  rdfs:comment "This property is used to indicates the current and historical value of a skos:notation. It is a property of the class euvc:XlNotation which reifies notation of a resource."@en ;
  rdfs:domain euvoc:XlNotation ;
  rdfs:range rdfs:Literal ;
.
euvoc:xlDefinition
  rdf:type owl:ObjectProperty ;
  rdfs:comment "Relates a resource to the current and historical values of a skos:note."@en ;
  rdfs:range euvoc:XlNote ;
  rdfs:subPropertyOf euvoc:xlNote ;
.
euvoc:xlEditorialNote
  rdf:type owl:ObjectProperty ;
  rdfs:comment "This property is a reified version of the skos:editorialNote" ;
  rdfs:label "xl editorial note" ;
  rdfs:range euvoc:XlNote ;
  rdfs:subPropertyOf euvoc:xlNote ;
  skos:prefLabel "xl editorial note" ;
.
euvoc:xlGetsReportingFrom
  rdf:type owl:ObjectProperty ;
  rdfs:comment "Current value and historical values of the reporting relationship."@en ;
  rdfs:range euvoc:XlSemanticRelation ;
  owl:inverseOf euvoc:xlReportsTo ;
.
euvoc:xlHasSubOrganization
  rdf:type owl:ObjectProperty ;
  rdfs:comment "Relates an Organization to the current and historical values of org:hasSubOrganization."@en ;
  rdfs:domain org:Organization ;
  rdfs:range euvoc:XlSemanticRelation ;
.
euvoc:xlHistoryNote
  rdf:type owl:ObjectProperty ;
  rdfs:comment "This property is a reified version of the skos:historyNote" ;
  rdfs:label "xl history note" ;
  rdfs:range euvoc:XlNote ;
  rdfs:subPropertyOf euvoc:xlNote ;
  skos:prefLabel "xl history note" ;
.
euvoc:xlNotation
  rdf:type owl:ObjectProperty ;
  rdfs:comment "Relates a resource to a Notation value."@en ;
  rdfs:range euvoc:XlNotation ;
.
euvoc:xlNote
  rdf:type owl:ObjectProperty ;
  rdfs:comment "This property is used to indicates the current and historical value of a note, for example a skos:note"@en ;
  rdfs:range euvoc:XlNote ;
.
euvoc:xlNumericalValue
  rdf:type owl:DatatypeProperty ;
  rdfs:comment "This property is used to indicates the current and historical value of a numerical property. It is a property of euvoc:XlNumericalValue which reifies a numerical property of a resource."@en ;
  rdfs:domain euvoc:XlNumericalValue ;
  rdfs:range xsd:integer ;
  owl:deprecated "true"^^xsd:boolean ;
.
euvoc:xlObject
  rdf:type owl:ObjectProperty ;
  rdfs:comment "When a semantic relationship is reified with euvoc:XlSemanticRelation (used for org:subOrganization or skos:broader for example), this property indicates the object of the relationship. The target of the relationship is indicated with the property euvo::xlTarget."@en ;
  rdfs:domain euvoc:XlSemanticRelation ;
  rdfs:range owl:Thing ;
.
euvoc:xlOrder
  rdf:type owl:ObjectProperty ;
  rdfs:comment "Current value and historical values of the numerical value giving the order of the organization among its sibling organizations but also sibling memberships."@en ;
.
euvoc:xlPositionComplement
  rdf:type owl:ObjectProperty ;
  rdfs:comment "actual and historical values of the position complemment."@en ;
  rdfs:range euvoc:XlNote ;
.
euvoc:xlProtocolLevel
  rdf:type owl:ObjectProperty ;
  rdfs:comment "Current value and historical values of the protocol-level."@en ;
  rdfs:domain org:Organization ;
  rdfs:range euvoc:XlNumericalValue ;
.
euvoc:xlReportsTo
  rdf:type owl:ObjectProperty ;
  rdfs:comment "Current value and historical values of the reporting relationship."@en ;
  rdfs:range euvoc:XlSemanticRelation ;
.
euvoc:xlScopeNote
  rdf:type owl:ObjectProperty ;
  rdfs:comment "This property is a reified version of the skos:scopeNote" ;
  rdfs:label "xl scope note" ;
  rdfs:range euvoc:XlNote ;
  rdfs:subPropertyOf euvoc:xlNote ;
  skos:prefLabel "xl scope note" ;
.
euvoc:xlSubOrganizationOf
  rdf:type owl:ObjectProperty ;
  rdfs:comment "Relates an Organization to the current and historical values of org:subOrganizationOf"@en ;
  rdfs:domain org:Organization ;
  rdfs:range euvoc:XlSemanticRelation ;
.
euvoc:xlTarget
  rdf:type owl:ObjectProperty ;
  rdfs:comment "When a semantic relationship is reified with euvoc:XlSemanticRelation (used for org:subOrganization or skos:broader for example), this property indicates the target of the relationship. The object of the relationship is indicated with the property euvo:xlObject."@en ;
  rdfs:domain euvoc:XlSemanticRelation ;
  rdfs:range owl:Thing ;
.
euvoc:xlTypeValue
  rdf:type owl:ObjectProperty ;
  rdfs:comment "Value of a Type when reified in the class euvo:XlType used to keep historical value of a type (used for org:classification historical values)."@en ;
  rdfs:domain euvoc:XlType ;
  rdfs:range skos:Concept ;
.
